Also expose hash_st in Blake2 wrapper

code/hash/Hacl.Hash.Blake2.fst
@@ -40,6 +40,7 @@ let update_last_blake2b_32 s prev input input_len =
 
 let finish_blake2b_32 s dst = BlB32.blake2b_finish (hash_len Blake2B) dst s
 
+let hash_blake2b_32 input input_len dst = BlB32.blake2b 64ul dst input_len input 0ul (null #MUT uint8)
 
 // Blake2s_32
 
@@ -68,6 +69,7 @@ let update_last_blake2s_32 s prev input input_len =
 
 let finish_blake2s_32 s dst = BlS32.blake2s_finish (hash_len Blake2S) dst s
 
+let hash_blake2s_32 input input_len dst = BlS32.blake2s 32ul dst input_len input 0ul (null #MUT uint8)
 
 // Blake2s_128
 
@@ -96,6 +98,7 @@ let update_last_blake2s_128 s prev input input_len =
 
 let finish_blake2s_128 s dst = BlS128.blake2s_finish (hash_len Blake2S) dst s
 
+let hash_blake2s_128 input input_len dst = BlS128.blake2s 32ul dst input_len input 0ul (null #MUT uint8)
 
 // Blake2b_256
 
@@ -123,3 +126,5 @@ let update_last_blake2b_256 s prev input input_len =
   ST.pop_frame()
 
 let finish_blake2b_256 s dst = BlB256.blake2b_finish (hash_len Blake2B) dst s
+
+let hash_blake2b_256 input input_len dst = BlB256.blake2b 64ul dst input_len input 0ul (null #MUT uint8)
